<?xml version="1.0" encoding="UTF-8"?>

<!-- This is the main course file for ... . It is used to generate all the public facing course materials so those can be hosted online.  -->

  <!-- Include common macros etc: -->

<worksheet xml:id="week5-handout">
  <title>Week 5 Handout- Series Solution-Part 1</title>

    <introduction>
        <statement> <p>
        We will discuss the following topics related to <term> Series Solution</term>:
      <ul>
        <li> <p>Week 5: Power Series about Ordinary Points and Singular Points (Section 5.1-5.2) </p>   </li>
        <li> <p>Week 6-7: Orthogonal Functions (Section 12.1), Legendre Function (Section 5.3), Fourier Series (Section 12.2-12.3)  </p> </li>

      </ul>  </p>
        </statement>

    </introduction>
  <definition xml:id="def-power-series">
    <statement>
      <p> A <term>power series</term> in <m>x-a</m> is an <alert>infinite series</alert> of the form
        <md xml:id="eq-series" number="yes">
          \sum_{n=0}^\infty c_n(x-a)^n=c_0+c_1(x-a)+c_2(x-a)^2+\cdots.
        </md>
        It is also called a <term>power series centered at <m>a</m>.</term>
      </p>
    </statement>
  </definition>
  <remark>
    <statement>
      <p>
    A few issues are important to consider when using a series:
    <ul>
      <li> <p> Is the series <alert>convergent</alert>?  </p> </li>
      <li> <p> If the series is convergent,
        <ul>
          <li> <p> What is the radius of convergence? 
            That is the same question as "What is the interval of convergence?".   </p>     </li>
          <li> <p> Is it convergent absolutely? Is it convergent pointwisely?  </p>    </li>
          <li> <p> Is it convergent to the function we are looking for? 
            Are the derivatives or the anti-derivatives of the series the same with the derivatives or the anti-derivatives
          of the function we are looking for?</p>  </li>
        </ul>   </p> </li>
      </ul> 
      
      Why is constructing a series solution important?
      <ul>
        <li><p> Iterative </p></li>
        <li><p> Truncated Series vs Error </p>
        </li>
      </ul>
      </p>
    </statement>
  </remark>
  <definition xml:id="def-analytic">
    <statement>
      <p>A function <m>f</m> is said to be <alert>analytic at a point <m>a</m></alert>
     if it can be represented by a power series in <m>x-a</m> with either a positive 
     or an infinite radius of convergence.   </p></statement>
    </definition>
  <example>
    <statement>
      <p>Find the radius of convergence and interval of convergence for the given power series.
      <ol>
        <li> <p>      <m> \sum_{n=1}^\infty \frac{3^n}{n}x^{n-1}</m>     </p>    </li>
        <li> <p>      <m>\sum_{m=1}^\infty \frac{2^m}{(m-1)!}(x+1)^{m+2}</m> </p> </li>
      </ol>
      </p>
    </statement>
    <solution component="inst">
      <p>
        <ol>
          <li> <p> Use Ratio Test: <m>\frac{a_{k+1}}{a_k}</m>:   
          <md>
            \frac{a_{k+1}}{a_k}=\frac{\frac{3^{k+1}}{k+1}x^{(k+1)-1}}{\frac{3^k}{k}x^{k-1}}=\frac{3kx}{k+1}
          </md>
          <md>
            \lim_{k\rightarrow\infty}\left|\frac{3kx}{k+1}\right|=|3x|
          </md>
          For an infinite geometric series to converge, the magnitude of the ratio must be less than 1.
          Thus, <m>|3x|\lt 1.</m>  That gives us the radius of convergence of <m>\frac{1}{3}.</m>
          <md>|x|\lt \frac{1}{3}\Rightarrow \frac{-1}{3}\lt x\lt \frac{1}{3}.</md>
          Next, check whether the series converges at <m>x=\frac{-1}{3}</m> and <m>x=\frac{1}{3}.</m>
          <ul>
            <li> <p> At <m>x=\frac{-1}{3},</m> the series becomes
            <md>
              <mrow>
              \sum_{n=1}^{\infty}\frac{3^n}{n}\left(\frac{-1}{3}\right)^{n-1}=\amp 3\sum_{n=1}^{\infty}\frac{ (-1)^{n-1}}{n}</mrow>
              <mrow>=\amp 3\left(\frac{1}{1}-\frac{1}{2}+\frac{1}{3}-\frac{1}{4}+\cdots\right)  </mrow>
            </md>
            By the <term>Alternating Series Test</term>, the series converges.
                  </p> </li>
            <li><p>   At <m>x=\frac{1}{3}</m>, the series becomes
            <md>  \sum_{n=1}^{\infty}\frac{3^n}{n}\left(\frac{1}{3}\right)^{n-1}=3\sum_{n=1}^\infty \frac{1}{n}
            </md>
            By the <term>Direct Comparison Test</term>, the series diverges.
                 </p>   </li>
          </ul>
          Thus the convergence interval is <m>\left[-\frac{1}{3},\frac{1}{3}\right).</m> </p> </li>
          <li> <p><md>
            \frac{\frac{2^{m+1}}{m!}(x+1)^{m+3}}{\frac{2^m}{(m-1)!}(x+1)^{m+2}}=\frac{2(x+1)}{m}</md> 
            Since <m> \lim_{m\rightarrow\infty} \left|\frac{2}{m}\right|=0  </m>, the radius of convergence is <m>\infty</m> 
            and the interval of convergence is <m>(-\infty,\infty).</m> </p> </li>
        </ol>
        
      </p>
    </solution>
  </example>
  <remark xml:id="rem-power-series">
    <statement>
      <p>  <alert>Taylor series</alert> centered at <m>a=0</m> is also called <alert>Maclaurin series</alert>.
        The five functions below are <term>analytic</term> at <m>a=0.</m> 
        
          <title>Power Series of Basic Functions</title>
          <tabular>
            <row>
              <cell><alert>Power Series</alert></cell> <cell><alert>Interval of Convergence</alert></cell>
            </row>
            <row>
              <cell><m>e^x=1+\frac{x}{1!}+\frac{x^2}{2!}+\cdots=\sum_{n=0}^\infty \frac{x^n}{n!}</m></cell>
               <cell><m>(-\infty, \infty)</m></cell>
            </row>
            <row>
              <cell><m>\cos x=1-\frac{x^2}{2!}+\frac{x^4}{4!}-\cdots=\sum_{n=0}^\infty \frac{(-1)^nx^{2n}}{(2n)!}</m></cell>
              <cell><m>(-\infty,\infty)</m></cell>
            </row>
            <row>
              <cell><m>\sin x=x-\frac{x^3}{3!}+\frac{x^5}{5!}-\cdots=\sum_{n=0}^\infty \frac{(-1)^nx^{2n+1}}{(2n+1)!}</m></cell>
              <cell><m>(-\infty,\infty)</m></cell>
            </row>
            <row>
              <cell><m>\ln(x+1)=x-\frac{x^2}{2}+\frac{x^3}{3}-\cdots=\sum_{n=1}^\infty\frac{(-1)^{n+1}x^n}{n}</m></cell>
              <cell><m> (-1,1]</m></cell>
            </row>
            <row>
              <cell><m>\frac{1}{1-x}=1+x+x^2+x^3+\cdots=\sum_{n=1}^\infty x^n</m></cell>
              <cell><m>(-1,1)</m></cell>
            </row>
          </tabular>
        </p>
    </statement>
  </remark>
  <example>
    <statement>
      <p> Using the power series in the Remark, find the first 4 terms 
        of a power series in <m>x</m> for each function below.
        <ol>
          <li> <p>  <m>\sin x \cos x</m>      </p>    </li>
          <li> <p>  <m>\frac{1}{\sin x}</m>     </p> </li>
        </ol>
      </p>
    </statement>
    <solution component="inst">
      <p><ol>
        <li><p> Expanding the product, it becomes
          <md>
            <mrow> \amp \sin x\cos x  </mrow>
            <mrow>=\amp\left(1-\frac{x^2}{2!}+\frac{x^4}{4!}-\frac{x^6}{6!}+\cdots\right)
              \left(x-\frac{x^3}{3!}+\frac{x^5}{5!}-\frac{x^7}{7!}+\cdots\right) </mrow>
            <mrow>=\amp x-\frac{x^3}{3!}+\frac{x^5}{5!}-\frac{x^7}{7!}+\cdots-\frac{x^3}{2!}+\frac{x^5}{2!3!}-\frac{x^7}{2!5!}+\cdots </mrow>
            <mrow>=\amp x+\left(-\frac{1}{6}-\frac{1}{2}\right)x^3+\left(\frac{1}{5!}+\frac{1}{2!3!}+\frac{1}{4!}\right)x^5</mrow>
            <mrow> \amp \left(-\frac{1}{7!}-\frac{1}{2!5!}-\frac{1}{4!3!}\right)x^7+\cdots </mrow>

          </md>  </p>       </li>
          <li>
            <p> Cannot directly do division, need other method.
              
            </p>
          </li>
      </ol>
        
      </p>
    </solution>
  </example>
  <example>
    <statement>
      <p>Verify by direct substituion that the given power series 
        is a particular solution of the indicated differential equation.
        <md xml:id="eq2-sub-series" number="yes">
          y=\sum_{n=1}^\infty \frac{(-1)^{n+1}}{n}x^{n}, (x+1)y''+y'=0</md>
      </p>
    </statement>
    <solution component="inst">
      <p> <md> 
          <mrow> y=\amp \sum_{n=1}^{\infty}\frac{(-1)^{n+1}}{n}x^n\amp= x-\frac{1}{2}x^2+\frac{1}{3}x^3-\frac{1}{4}x^4+\cdots</mrow>
          <mrow> y'=\amp \sum_{n=0}^{\infty}(-1)^{n}x^n\amp= 1-x+x^2-x^3+x^4-\cdots </mrow>
          <mrow> y''=\amp \sum_{n=0}^{\infty} (-1)^{n+1}x^n (n+1)\amp= -1+2x-3x^2+4x^3+\cdots</mrow>
      </md>
      <md>
        <mrow> \amp (x+1)y''+y' </mrow>
        <mrow> = \amp  (x+1)\sum_{n=0}^{\infty} (-1)^{n+1}x^n (n+1)+\sum_{n=0}^{\infty}(-1)^{n}x^n </mrow>
        <mrow> = \amp \sum_{n=0}^{\infty} (-1)^{n+1}x^{n+1} (n+1)+\sum_{n=0}^{\infty} (-1)^{n+1}x^n (n+1)+\sum_{n=0}^{\infty}(-1)^{n}x^n </mrow>
        <mrow> = \amp \sum_{k=1}^\infty (-1)^kkx^k+\sum_{n=0}^{\infty} (-1)^{n+1}x^n (n+1)+\sum_{n=0}^{\infty}(-1)^{n}x^n </mrow>
        <mrow> = \amp \sum_{k=1}^\infty\left[k(-1)^k+(-1)^{k+1}(k+1)+(-1)^k\right]x^k+(-1)^1\cdot 1\cdot x^0+ (-1)^0\cdot x^0</mrow>
        <mrow> = \amp \sum_{k=1}^\infty(-1)^k\left[k-(k+1)+1\right]x^k+0 </mrow>
        <mrow> =\amp \sum_{k=1}^\infty (-1)^k\cdot 0\cdot x^k</mrow>
        <mrow> =\amp 0</mrow>
      </md>
      
        
      </p>
    </solution>
  </example>
  <definition xml:id="def-ordinary-point">
    <statement>
      <p>The standard form of a linear second order differential equation is defined as
        <equation xml:id="eq-DE-standard"> 
        <md>
          y''+P(x)y'+Q(x)y=0.
        </md> 
      </equation>  
        A point <m>x_0</m> is said to be an <term>ordinary point</term> of the differential equation
        if both <m>P(x)</m> and <m>Q(x)</m> in the standard form are <term>analytic</term> at <m>x_0.</m>
        A point that is not an ordinary point is said to be a <term>singular point</term> of the equation.
      </p>
    </statement>
  </definition>
  <example>
    <statement>
      <p>Identify all ordinary points and singular points of  <md>(x^2-4x-5)y''+2xy'+3y=0.</md></p>
    </statement>
    <solution>
      <p>Convert to the standard form:
        <md>
          y''+\frac{2x}{x^2-4x-5}y'+\frac{3}{x^2-4x-5}y=0
        </md>
        <md>
          \Rightarrow P(x)=\frac{2x}{x^2-4x-5} \mbox{ and } Q(x)=\frac{3}{x^2-4x-5}    </md>
        <md>
          x^2-4x-5=0\Rightarrow (x-5)(x+1)=0\Rightarrow x=5 \mbox{ or } x=-1
        </md>
        <m>P(x)</m> and <m>Q(x)</m> are analytic at all real numbers, except <m>5</m> or <m>-1.</m>
        Thus singular points for the given DE are <m>\{-1,5\}</m> and the ordinary points are 
        <m>x\neq -1</m> and <m>x\neq 5,</m> i.e., <m>(-\infty, -1)\bigcup(-1,5)\bigcup(5,\infty).</m>

        
      </p>
    </solution>
  </example>
  <theorem xml:id="thm-existence-power-solution">
    <statement>
      <p>If <m>x=x_0</m> is an ordinary point of a 2nd order linear differential equation, 
        we can always find 2 linearly independent solutions in the form of 
        a power series centered at <m>x_0</m>; that is <m>y=\sum_{n=0}^\infty c_n(x-x_0)^n,</m> 
        called <alert>a solution about the ordinary point <m>x_0.</m></alert> 

        A series solution converges at least on some interval defined by 
        <m>|x-x_0|\lt R,</m> where <m>R</m> is the distance from <m>x_0</m> 
        to be the closest singular point.   </p>
    </statement>
  </theorem>
  <example>
    <statement>
      <p>Find a power series solution of each given differential equation about the ordinary point 
        <m>x=0</m> and a lower bound for the radius of convergence.
        <ol>
          <li> <p> <m>y''+x^2y'+xy=0</m>    </p>     </li>
          <li> <p> <m>(x^2+2)y''+3xy'-y=0</m>      </p>
          </li>
        </ol>      </p>
       </statement>
       <solution>
        <p>
          <ol>
            <li> <p> Considering <m>y''+x^2y'+xy=0,</m> <m>x=0</m> is an ordinary point. 
              By <xref ref="thm-existence-power-solution"/>, there exists a solution <m>y(t)</m>
              in the form of <md> y(t)=\sum_{n=0}^\infty c_n(x-0)^n=\sum_{n=0}^\infty c_n x^n.</md> 
                <md> 
                  <mrow>y'= \amp \sum_{n=1}^\infty c_nnx^{n-1} </mrow>
                  <mrow>y''=\amp \sum_{n=2}^\infty c_nn(n-1)x^{n-2} </mrow>
                </md>
                <md>
                  <mrow> \amp y''+x^2y'+xy=0 </mrow>
                  <mrow>\Rightarrow \amp \sum_{n=2}^\infty c_nn(n-1)x^{n-2}+x^2\sum_{n=1}^\infty c_nnx^{n-1}+x\sum_{n=0}^\infty c_n x^n=0 </mrow>
                  <mrow>\Rightarrow \amp\sum_{n=2}^\infty c_nn(n-1)x^{n-2}+\sum_{n=1}^\infty c_nnx^{n+1}+\sum_{n=0}^\infty c_n x^{n+1}=0  </mrow>
                  <mrow> \Rightarrow \amp \sum_{k=0}^\infty c_{k+2}(k+2)(k+1)x^k+\sum_{k=2}^\infty (k-1)c_{k-1}x^k+\sum_{k=1}^\infty c_{k-1}x^k=0 </mrow>
                  <mrow>\Rightarrow \amp 2c_2+(c_0+6c_3)x+\sum_{k=2}^\infty \left(c_{k-1}\cdot k+(k+2)(k+1)c_{k+2}\right)x^k =0</mrow>
                </md>
              <md>
                <mrow> 2c_2=0 \amp \Rightarrow c_2=0 </mrow>
                <mrow> c_0+6c_3=0 \amp \Rightarrow c_3=-\frac{1}{6}c_0 </mrow>
                <mrow> kc_{k-1}+(k+2)(k+1)c_{k+2}=0 \amp \Rightarrow c_{k+2}=-\frac{kc_{k-1}}{(k+2)(k+1)}, k\geq 2 </mrow>
              </md>
              From the above relations, there are two free variables <m>c_0</m> and <m>c_1,</m> which
              generate two sequences of coefficients, <m>\{c_0, c_3,c_6,\ldots\}</m> and 
              <m>\{c_1, c_4, c_7,\ldots\}.</m>  Thus, we have
              <md>
                <mrow>y_1(x)= \amp \sum_{n=0}^\infty c_{3n}x^{3n}, \mbox{ where } c_{3(n+1)}=\frac{-(3n+1)c_3n}{(3n+3)(3n+2)},</mrow>
                <mrow>y_2(x)= \amp \sum_{n=0}^\infty c_{3n+1}x^{3n+1}, \mbox{ where } c_{3n+4}=\frac{-(3n+2)c_{3n+1}}{(3n+4)(3n+5)}, </mrow>
                <mrow>\Rightarrow \amp  y(x)= a_1y_1(x)+a_2y_2(x).</mrow>
              </md>
              
              </p>   </li>
          </ol>
        </p>
       </solution>
  </example>

  <definition xml:id="def-regular-singular">
    <statement>
      <p>A singular point <m>x_0</m> is said to be a <alert>regular singular point</alert>
         of the 2nd order linear differential equation if <term> the functions <m>p(x)=(x-x_0)P(x)</m>
           and <m>q(x)=(x-x_0)^2Q(x)</m> are both analytic at <m>x_0.</m></term>
            A singular point is <term> not regular</term> is said to be an  <term>irregular singular point</term>
             of the equation.  </p>
    </statement>
  </definition>
  <example> <statement>
    <p>Determine the singular points of each given differential equation. 
      Classify each singular point as regular or irregular.
      <ol>
        <li> <p> <m>x^3y''+3x^2y'+6y=0</m>      </p>   </li>
        <li> <p> <m>(x^2-16)^2y''+(x-4)y'+5y=0</m>     </p> </li>
      </ol>
    </p>
  </statement>  
  <solution component="inst">
    <p><ol>
      <li> <p><md> y''+\frac{3x^2}{x^3}y'+\frac{6}{x^3}y=0 \Rightarrow P(x)=\frac{3x^2}{x^3}, Q(x)=\frac{6}{x^3} </md>
        <m>\Rightarrow x=0</m> is a singular point.  Since <m>x=0</m> is not analytic for <m>x^2Q(x),</m>
        <m>x=0</m> is an <term>irregular singular point.</term>  </p> </li>
      <li><p>
        <md><mrow> y''+\frac{(x-4)}{(x^2-16)^2}y'+\frac{5}{(x^2-16)^2}y=0</mrow>
          <mrow> \Rightarrow P(x)=\frac{(x-4)}{(x^2-16)^2}, Q(x)=\frac{5}{(x^2-16)^2} </mrow>  </md>
        <m>x=4</m> is a regular singular point and <m>x=-4</m> an irregular singular point.
            </p>
      </li>
    </ol>
      
    </p>
  </solution> 
  </example>
  <theorem xml:id="thm-Frobenius">
    <title>Method of Frobenius</title> 
    <statement>
      <p>If <m>x=x_0</m> is a regular singular point of the 2nd order linear differential equation, 
        then there exists at least one nonzero solution of the form 
      <equation xml:id="froben">
        <md> y=(x-x_0)^r\sum_{n=0}^\infty c_n(x-x_0)^n=\sum_{n=0}^\infty c_n(x-x_0)^{n+r},</md>
      </equation>
        where the number <m>r</m> is a constant to be determined. 
        The series will converge at least on some interval defined by <m>0\lt x-x_0\lt R.</m>
      </p>
    </statement>
  </theorem>
  <example>
    <statement>
      <p>Find a solution of the form <m>y=\sum_{n=0}^\infty c_nx^{n+r}</m> for
        <md> 4xy''+2y'-y=0</md>      
      </p>
    </statement>
    <solution component="inst">
      <p> <m>y''-\frac{2}{4x}y'-\frac{1}{4x}y=0 \Rightarrow P(x)=\frac{-1}{2x}, Q(x)=-\frac{1}{4x}.</m>
        <m>\Rightarrow p(x)=(x-0)P(x), q(x)=(x-0)^2Q(x)</m> are both analytic at <m>x=0.</m> Thus <m>x=0</m> 
        is a regular singular point.

        <md>
          <mrow> y=\amp \sum_{n=0}^\infty c_nx^{n+r}</mrow>
          <mrow> y'=\amp \sum_{n=0}^\infty c_n(n+r)x^{n+r-1} </mrow>
          <mrow> y''=\amp \sum_{n=0}^\infty c_n(n+r)(n+r-1)x^{n+r-2} \amp </mrow>
        </md>
        <md>
          <mrow>\amp 4xy''+2y'-y </mrow>
          <mrow>= \amp 4\sum_{n=0}^\infty c_n(n+r)(n+r-1)x^{n+r-1} </mrow>
          <mrow> \amp +2\sum_{n=0}^\infty c_n(n+r)x^{n+r-1} - \sum_{n=0}^\infty c_nx^{n+r}</mrow>
          <mrow> =\amp \sum_{n=0}^\infty\left[c_n(n+r)(4(n+r-1)+2)\right]x^{n+r-1}- \sum_{n=0}^\infty c_nx^{n+r}</mrow>
          <mrow> =\amp x^r\left[c_0r(4r-2)x^{-1}+\sum_{n=1}^\infty c_n(n+r)(4n+4r-2)x^{n-1}-\sum_{n=0}^\infty c_nx^n\right]</mrow>
          <mrow> = \amp x^r\left[c_0r(4r-2)x^{-1}+\sum_{n=0}^\infty \left[c_{n+1}(n+r+1)(4n+4r+c)-c_n\right]x^n\right]</mrow>
        </md>
        <md>
          <mrow> \mbox{lowest degree in } x = x^{-1} :\mbox{ } \amp   c_nr(4r-2)=0 </mrow>
          <mrow> x^{n}:\mbox{ } \amp  c_{n+1}(n+r+1)(4n+4r+2)-c_n=0 </mrow>
        </md>
        If <m>c_0=0</m>, it produces the trivial solution <m>y(x)\equiv 0.</m>  For nontrivial solution (<m>c_0\neq 0</m>),
        <md>
          r(4r-2)=0 \Rightarrow r_1=0, r_2=\frac{1}{2}.
        </md>
        <m>r(4r-2)=0</m> is called an <term>Indicial Equation</term> and <m>r_1=0</m> and <m> r_2=\frac{1}{2}</m> 
        are called <term>indicial roots.</term>  Next,
        <md>
           <mrow> \amp c_{n+1}(n+r+1)(4n+4r+2)-c_n=0, n=0,1,2,\ldots </mrow>
           <mrow> \Rightarrow \amp c_{n+1}=\frac{c_n}{(n+r+1)(4n+4r+2)}</mrow>
        </md>
        <md>
          <mrow>r_1=0 \amp\Rightarrow c_{n+1}=\frac{c_n}{(n+1)(4n+2)}, n=0,1,2,\ldots \rightarrow y_1(x) </mrow>
          <mrow>r_2=\frac{1}{2} \amp \Rightarrow c_{n+1}\frac{c_n}{\left(n+\frac{3}{2}\right)\left(4n+4\right)}, n=0,1,2,\ldots, \rightarrow y_2(x) </mrow>
        </md>
        <md>
          <mrow> y_1(x)= \amp \sum_{n=0}^\infty c_nx^n, \mbox{ where }c_{n+1}=\frac{c_n}{(n+1)(4n+2)} </mrow>
          <mrow> y_2(x)= \amp \sum_{n=0}^\infty b_nx^{n+\frac{1}{2}}, \mbox{ where }b_{n+1}=\frac{b_n}{\left(n+\frac{3}{2}\right)\left(4n+2\right)} </mrow>
          <mrow> y(x)= \amp a_1y_1(x)+a_2y_2(x) </mrow>
        </md>       
      </p>
    </solution>
  </example>
  <definition xml:id="def-indicial">
    <statement>
      <p>After substituting <m>y=\sum_{n=0}^\infty c_nx^{n+r}</m>
         into the given differential equation and simplifying, the <term>indicial equation</term>
          is a equation in <m>r</m> that results from equating the total coefficient 
          of the lowest power of <m>x</m> to zero. The solutions to the indicial equation 
          are called <term>indicial roots</term>, or <term>exponents</term> of 
          the singularity <m>x=0.</m>

          When the given differential equations are in the standard form of the 2nd order DE, 
          the indicial equation is quadratic.        
      </p>
    </statement>
  </definition>
  <remark>
    <statement>
      <p> 3 Cases of <m>r_1</m> and <m>r_2</m>:
        <ul> <li>  <p><term>Case I:</term> <m>r_1</m> and <m>r_2</m> are distinct 
                  and do not differ by an integer 
                <md><mrow>y_1(x)=\amp \sum_{n=0}^\infty c_nx^{n+r_1},</mrow>
                  <mrow> y_2(x)=\amp \sum_{n=0}^\infty b_nx^{n+r_2}</mrow> </md></p>    </li>
              <li><p><term>Case II:</term> <m>r_1-r_2=N</m>, where <m>N</m> is a positive integer 
              <md> 
                <mrow> y_1(x)=\amp \sum_{n=0}^\infty c_nx^{n+r_1}, c_0\neq 0 </mrow>
                <mrow>y_2(x)=\amp c y_1(x)\ln(x)+\sum_{n=0}^\infty b_nx^{n+r_2}, b_0\neq 0, c \mbox{ is a constant.}</mrow> </md></p>  </li>    
              <li><p><term>Case III:</term>  <m>r_1=r_2</m>    
              <md> 
                <mrow>y_1(x)=\amp \sum_{n=0}^\infty c_nx^{n+r_1}, c_0\neq 0</mrow>
                <mrow>y_1(x)=\amp y_1(x)\ln(x)+\sum_{n=0}^\infty b_nx^{n+r_1}</mrow>
              </md> </p></li>
        </ul>
      </p>
    </statement>
  </remark>
  <example>
    <statement>
      <p> For each given differential equations, show that the indicial roots of 
        the singularity do not differ by an integer, use the method of Frobenius to 
        obtain 2 linearly independent series solution about <m>x=0,</m> and 
        form the general solution on the interval <m>(0,\infty).</m>
          <ol>
            <li>   <p>  <m>3xy''+(2-x)y'-y=0</m>       </p>  </li>
            <li>  <p><m>9x^2y''+9x^2y'+2y=0</m>        </p>     </li>
          </ol>
      </p>
    </statement>
    <solution component="inst">
      <p><ol>
        <li><p> <m>3xy''+(2-x)y'-y=0 \Rightarrow y''+\frac{2-x}{3x}y'-\frac{1}{3x}y=0</m> 
        <m>\Rightarrow P(x)=\frac{2-x}{3x}, Q(x)=\frac{-1}{3x}.</m> Thus, <m>x=0</m> is a singular point.
        Since <m>p(x)=xP(x)</m> and <m>q(x)=x^2Q(x)</m>  are both analytic at <m>x=0,</m>  <m>x=0</m>
      is a regular singular point.  Let <m>y(x)=\sum_{n=0}^\infty c_nx^{n+r}</m>.
       <md>
        <mrow> \amp 3xy''+(2-x)y'-y </mrow>
        <mrow>= \amp 3\sum_{n=0}^\infty c_n(n+r)(n+r-1)x^{n+r-1}</mrow>
        <mrow>\amp + (2-x)\sum_{n=0}c_n(n+r)x^{n+r-1}-\sum_{n=0}^\infty c_nx^{n+r} </mrow>
        <mrow>= \amp \sum_{n=0}^\infty \left[3(n+r)(n+r-1)c_n+2(n+r)c_n\right]x^{n+r-1}</mrow>
          <mrow> \amp -\sum_{n=0}^\infty \left[(2n+r)c_n+c_n\right]x^{n+r}  </mrow>
          <mrow> =\amp 0</mrow>
       </md>
       <md>
        <mrow>3r(r-1)c_0+2rc_0=0 \amp \Rightarrow 3r(r-1)+2r=0\Rightarrow 3r^2-r=0</mrow>
        <mrow> \amp \Rightarrow r=0 \mbox{ or } r=\frac{1}{3} </mrow>
       </md>
       <md>
        <mrow> \left[3(n+r+1)(n+r)+2(n+r+1)\right]c_{n+1}-(2n+r+1)c_n =0</mrow>
        <mrow> \Rightarrow  c_{n+1}=\frac{(2n+r+1)c_n}{(n+r+1)(3n+3r+2)} </mrow>
       </md>
       <md>
        <mrow>y_1(x)= \amp \sum_{n=0}^\infty c_nx^n, \mbox{ where }c_{n+1}=\frac{(2n+1)c_n}{(n+1)(3n+2)}  </mrow>
        <mrow>y_2(x)= \amp \sum_{n=0}^\infty b_nx^{n+\frac{1}{3}}, \mbox{ where }b_{n+1}=\frac{\left(2n+\frac{4}{3}\right)b_n}{\left(n+\frac{4}{3}\right)\left(3n+3\right)}  </mrow>
        <mrow>\Rightarrow y(x)=\amp a_1y_1(x)+a_2y_2(x)</mrow>
       </md> 
       </p> </li>
       <li>
        <p>
          
        </p>
       </li>
      </ol>       
      </p>
    </solution>
  </example>
  <example>
    <statement>
      <p> The differential equation (DE) <m>x^4y''+\lambda y=0</m> has an irregular 
        singular point at <m>x=0.</m> 
        <ol>
          <li><p>  Show that the substitution <m>t=\frac{1}{x}</m> yields the DE 
            <md> \frac{d^2 y}{dt^2}+\frac{2}{t}\frac{dy}{dt}+\lambda y=0</md>
             which now has a regular singular point at <m>t=0.</m></p>   </li>
          <li> <p>Find two series solutions of the above equation about the 
            singular point <m>t=0.</m>         </p>    </li>
          <li>   <p> Express each solution of the original equation in terms of elementary functions.  </p></li>
          </ol>
      </p>
    </statement>
    <solution component="inst">
      <p><ol>
        <li> <p> <m>t=\frac{1}{x}\Rightarrow x=\frac{1}{t}\Rightarrow \frac{dx}{dt}=-t^{-2} \mbox{ and }\frac{d^2x}{dt^2}=2t^{-3}</m>
        <md>
          <mrow>\frac{dy}{dt} =\amp \frac{dy}{dx}\frac{dx}{dt} =\frac{dy}{dx}\left(-t^{-2}\right)</mrow>
          <mrow> \frac{dy}{dx}=\amp -t^2\frac{dy}{dt}  </mrow>
          <mrow> \frac{d^2y}{dt^2}=\amp \frac{d^2y}{dx^2}\left(\frac{dx}{dt}\right)^2+\frac{dy}{dx}\frac{d^2x}{dt^2} </mrow>
          <mrow> = \amp \frac{d^2y}{dx^2}\left(-t^{-2}\right)^2+\frac{dy}{dx}\left(2t^{-3}\right) </mrow>
          <mrow> = \amp  \frac{d^2y}{dx^2}\left(-t^{-2}\right)^2+\left(-t^2\frac{dy}{dt}\right)\left(2t^{-3}\right) </mrow>
          <mrow>\frac{d^2y}{dx^2}= \amp t^4\frac{d^2y}{dt^2}+2t^3\frac{dy}{dt}</mrow>
        </md>
        <md>
          <mrow>\amp x^4y''+\lambda y=0 </mrow>
          <mrow>\Rightarrow \amp \left(\frac{1}{t}\right)^4\left[t^4\frac{d^2y}{dt^2}+2t^3\frac{dy}{dt}\right]+\lambda y=0 </mrow>
          <mrow> \Rightarrow \amp \frac{d^2y}{dt^2}+\frac{2}{t}\frac{dy}{dt}+\lambda y=0 </mrow>
        </md>
        
             </p>  </li>
      </ol>
        
      </p>
    </solution>
  </example>

</worksheet>

